src/UntypedComp.v
@@ -5,18 +5,13 @@ Require Import StructTact.StructTactics.
 Require Import Utopia.
 Require Import Program.
 
+Require Import HList.
 
 Require SourceLang.
 Require Untyped.
 
 Module S := SourceLang.
 Module U := Untyped.
-
-Fixpoint member {A} {ty : A} {l} (m : S.member ty l) : nat :=
-  match m with
-  | S.Here => 0
-  | S.There m' => S (member m')
-  end.
 
 Definition elim_to_type_name {l cases target} (e : S.elim l cases target) : type_name :=
   match e with
@@ -27,14 +22,14 @@ Definition elim_to_type_name {l cases target} (e : S.elim l cases target) : type
 
 Definition compile {l ty} (e : S.expr l ty) : U.expr :=
   let fix go {l ty} (e : S.expr l ty) : U.expr :=
-      let fix go_hlist {l tys} (h : S.hlist (S.expr l) tys) : list U.expr :=
+      let fix go_hlist {l tys} (h : hlist (S.expr l) tys) : list U.expr :=
           match h with
-          | S.hnil => []
-          | S.hcons x h' => cons (go x) (go_hlist h')
+          | hnil => []
+          | hcons x h' => cons (go x) (go_hlist h')
           end
       in
       match e with
-      | S.Var v                   => U.Var (member v)
+      | S.Var v                   => U.Var (member_to_nat v)
       | S.Lam b                   => U.Lam (go b)
       | S.App e1 e2               => U.App (go e1) (go e2)
       | @S.Constr  _ _ _ c _ args => U.Constr c (go_hlist args)
@@ -42,42 +37,17 @@ Definition compile {l ty} (e : S.expr l ty) : U.expr :=
       end
   in go e.
 
-Fixpoint compile_hlist {l tys} (h : S.hlist (S.expr l) tys) : list U.expr :=
+Fixpoint compile_hlist {l tys} (h : hlist (S.expr l) tys) : list U.expr :=
   match h with
-  | S.hnil => []
-  | S.hcons x h' => cons (compile x) (compile_hlist h')
-  end.
-
-Fixpoint hmap_simple {A} {B : A -> Type} {C} (f : forall a, B a -> C) {l} (h : S.hlist B l) : list C :=
-  match h with
-  | S.hnil => []
-  | S.hcons x h' => cons (f _ x) (hmap_simple f h')
+  | hnil => []
+  | hcons x h' => cons (compile x) (compile_hlist h')
   end.
 
 Lemma compile_hlist_hmap_simple :
-  forall l tys (h : S.hlist (S.expr l) tys),
+  forall l tys (h : hlist (S.expr l) tys),
     compile_hlist h = hmap_simple (@compile l) h.
 Proof.
   induction h; simpl; auto using f_equal.
-Qed.
-
-Lemma nth_member_hget :
-  forall A (B : A -> Type) C (f : forall a, B a -> C) c l (h : S.hlist B l) t (m : S.member t l),
-    nth (member m) (hmap_simple f h) c = f _ (S.hget h m).
-Proof.
-  induction h; intros.
-  - destruct m using S.case_member_nil.
-  - destruct a, l, m using S.case_member_cons; simpl; auto.
-Qed.
-
-
-Lemma member_insert_member :
-  forall A (a1 a2 : A) l (m : S.member a1 l) n,
-    member (S.insert_member(ty' := a2) m n) =
-    if Compare_dec.lt_dec (member m) n then member m else S (member m).
-Proof.
-  induction m; simpl; intros; break_match; simpl; auto.
-  rewrite IHm. repeat break_if; auto; omega.
 Qed.
 
 Lemma compile_lift' :
@@ -85,19 +55,19 @@ Lemma compile_lift' :
     compile (S.lift'(ty' := ty') n e) = U.shift' n (compile e).
 Proof.
   refine (S.expr_mut_ind' _ _ _ _ _ _); intros; simpl.
-  - rewrite member_insert_member.
+  - rewrite member_to_nat_insert_member.
     break_if; auto.
   - f_equal.
     apply H with (n := (S n)).
   - f_equal; auto.
   - destruct ct;
-      repeat destruct args, H as [? args] using S.case_HForall_cons;
-      repeat destruct args, H using S.case_HForall_nil;
+      repeat destruct args, H as [? args] using case_HForall_cons;
+      repeat destruct args, H using case_HForall_nil;
       simpl; auto using f_equal, f_equal2.
   - unfold elim_to_type_name.
     destruct e;
-     repeat destruct cases, H as [? cases] using S.case_HForall_cons;
-     repeat destruct cases, H using S.case_HForall_nil;
+     repeat destruct cases, H as [? cases] using case_HForall_cons;
+     repeat destruct cases, H using case_HForall_nil;
      simpl; auto using f_equal, f_equal2.
 Qed.
 
@@ -109,48 +79,25 @@ Proof.
   apply compile_lift'.
 Qed.
 
-Lemma map_hmap_simple :
-  forall A (B : A -> Type) C D (f : forall a, B a -> C) (g : C -> D) l (hl : S.hlist B l),
-    map g (hmap_simple f hl) =
-    hmap_simple (fun a b => g (f a b)) hl.
-Proof.
-  induction hl; simpl; auto using f_equal.
-Qed.
-
-Lemma hmap_simple_hmap :
-  forall A (B C : A -> Type) D (f : forall a, B a -> C a) (g : forall a, C a -> D) l (hl : S.hlist B l),
-    hmap_simple g (S.hmap f hl) = hmap_simple (fun a b => g a (f a b)) hl.
-Proof.
-  induction hl; simpl; auto using f_equal.
-Qed.
-
-Lemma hmap_simple_ext :
-  forall A (B : A -> Type) C (f g : forall a, B a -> C) l (hl : S.hlist B l),
-    (forall a (b : B a), f a b = g a b) ->
-    hmap_simple f hl = hmap_simple g hl.
-Proof.
-  induction hl; simpl; auto using f_equal2.
-Qed.
-
 Theorem compile_subst :
-  forall l ty (e : S.expr l ty) l' (h : S.hlist (S.expr l') l),
+  forall l ty (e : S.expr l ty) l' (h : hlist (S.expr l') l),
     compile (S.subst e h) = U.multisubst' (hmap_simple (@compile l') h) (compile e).
 Proof.
   refine (S.expr_mut_ind' _ _ _ _ _ _); intros; simpl.
-  - now rewrite nth_member_hget.
+  - now rewrite nth_member_to_nat_hget.
   - f_equal. rewrite H. simpl. f_equal. f_equal.
     rewrite map_hmap_simple, hmap_simple_hmap.
     apply hmap_simple_ext.
     intros. apply compile_lift.
   - f_equal; auto.
   - destruct ct;
-      repeat destruct args, H as [? args] using S.case_HForall_cons;
-      repeat destruct args, H using S.case_HForall_nil;
+      repeat destruct args, H as [? args] using case_HForall_cons;
+      repeat destruct args, H using case_HForall_nil;
       simpl; auto using f_equal, f_equal2.
   - unfold elim_to_type_name.
     destruct e;
-      repeat destruct cases, H as [? cases] using S.case_HForall_cons;
-      repeat destruct cases, H using S.case_HForall_nil;
+      repeat destruct cases, H as [? cases] using case_HForall_cons;
+      repeat destruct cases, H using case_HForall_nil;
       simpl; auto using f_equal, f_equal2.
 Qed.
 
@@ -170,19 +117,23 @@ Qed.
 Hint Constructors U.step.
 
 Lemma compile_hlist_app :
-  forall l tys1 tys2 (h1 : S.hlist (S.expr l) tys1) (h2 : S.hlist (S.expr l) tys2),
-    compile_hlist (S.happ h1 h2) =
+  forall l tys1 tys2 (h1 : hlist (S.expr l) tys1) (h2 : hlist (S.expr l) tys2),
+    compile_hlist (happ h1 h2) =
     compile_hlist h1 ++ compile_hlist h2.
 Proof.
-  induction h1; simpl; auto using f_equal.
+  intros.
+  rewrite !compile_hlist_hmap_simple.
+  auto using hmap_simple_happ.
 Qed.
 
 Lemma compile_hlist_Forall_value :
-  forall l tys (args : S.hlist (S.expr l) tys),
-    S.HForall (fun ty e => S.value e) args ->
+  forall l tys (args : hlist (S.expr l) tys),
+    HForall (fun ty e => S.value e) args ->
     Forall U.value (compile_hlist args).
 Proof.
-  induction 1; simpl; auto using compile_value.
+  intros.
+  rewrite compile_hlist_hmap_simple.
+  eauto using HForall_Forall_hmap_simple, compile_value.
 Qed.
 
 Lemma compile_unroll' :
@@ -190,7 +141,7 @@ Lemma compile_unroll' :
     (mk_urec : U.expr -> U.expr)
     (mk_rec : S.expr l ty_rec -> S.expr l arg_rec),
     (forall e : S.expr l ty_rec, compile (mk_rec e) = mk_urec (compile e)) ->
-    forall (args : S.hlist (S.expr l) arg_tys)
+    forall (args : hlist (S.expr l) arg_tys)
     (case : S.expr l (S.arrow_all ty_rec arg_rec arg_tys ty))
     i,
     (forall j, nth_error arg_tys j = Some ty_rec ->
@@ -236,11 +187,11 @@ Qed.
 Lemma compile_eliminate :
   forall case_tys target_tyn arg_tys ty l c
     (e : S.elim case_tys (S.ADT target_tyn) ty)
-    (cases : S.hlist (S.expr l) case_tys)
+    (cases : hlist (S.expr l) case_tys)
     (ct : S.constr_type c arg_tys target_tyn)
-    (args : S.hlist (S.expr l) arg_tys),
-    compile (S.unroll args (S.hget cases (S.eliminate_case_type e ct)) (S.Elim e cases)) =
-    U.unroll_elim (compile (S.hget cases (S.eliminate_case_type e ct)))
+    (args : hlist (S.expr l) arg_tys),
+    compile (S.unroll args (hget cases (S.eliminate_case_type e ct)) (S.Elim e cases)) =
+    U.unroll_elim (compile (hget cases (S.eliminate_case_type e ct)))
                   c
                   (compile_hlist args)
                   (U.Elim target_tyn (compile_hlist cases)).
@@ -260,18 +211,11 @@ Proof.
     destruct j; simpl in *; try congruence.
 Qed.
 
-Lemma nth_error_hmap_simple_hget :
-  forall A (B : A -> Type) C (f : forall a, B a -> C) l (h : S.hlist B l) a (m : S.member a l),
-    nth_error (hmap_simple f h) (member m) = Some (f _ (S.hget h m)).
-Proof.
-  induction h; intros; dependent destruction m; simpl; auto.
-Qed.
-
 Lemma constructor_index_correct :
   forall case_tys target_tyn arg_tys ty c
     (e : S.elim case_tys (S.ADT target_tyn) ty)
     (ct : S.constr_type c arg_tys target_tyn),
-    member (S.eliminate_case_type e ct) = constructor_index c.
+    member_to_nat (S.eliminate_case_type e ct) = constructor_index c.
 Proof.
   dependent destruction e; dependent destruction ct; auto.
 Qed.
